% Created 2016-12-18 So 21:16
\documentclass[11pt]{article}
\usepackage[utf8]{inputenc}
\usepackage[T1]{fontenc}
\usepackage{fixltx2e}
\usepackage{graphicx}
\usepackage{longtable}
\usepackage{float}
\usepackage{wrapfig}
\usepackage{rotating}
\usepackage[normalem]{ulem}
\usepackage{amsmath}
\usepackage{textcomp}
\usepackage{marvosym}
\usepackage{wasysym}
\usepackage{amssymb}
\usepackage{hyperref}
\tolerance=1000
\usepackage{siunitx}
\usepackage{fontspec}
\sisetup{load-configurations = abbrevations}
\newcommand{\estimates}{\overset{\scriptscriptstyle\wedge}{=}}
\usepackage{mathtools}
\DeclarePairedDelimiter\abs{\lvert}{\rvert}%
\DeclarePairedDelimiter\norm{\lVert}{\rVert}%
\DeclareMathOperator{\Exists}{\exists}
\DeclareMathOperator{\Forall}{\forall}
\def\cvec#1{\left(\vcenter{\halign{\hfil$##$\hfil\cr \cvecA#1;;}}\right)}
\def\cvecA#1;{\if;#1;\else #1\cr \expandafter \cvecA \fi}
\renewcommand{\d}{\mathrm{d}}
\newcommand{\f}[2]{{\frac{#1}{#2}}}
\renewcommand{\v}[1]{\vec{#1}}
\usepackage{tikz}
\usetikzlibrary{calc,patterns,decorations.pathmorphing,decorations.markings}
\author{Robin Heinemann}
\date{\today}
\title{Experimentalphysik Übung (R. Weis)}
\hypersetup{
  pdfkeywords={},
  pdfsubject={},
  pdfcreator={Emacs 25.1.1 (Org mode 8.2.10)}}
\begin{document}

\maketitle
\tableofcontents


\section{Aufgabe 3}
\label{sec-1}
\[s_z = \frac{1}{2}a t^2 + v_0 t\]
\[s = v(t - t_v)\]
3 Möglichkeiten:
\begin{enumerate}
\item zu langsam
\item "zu" schnell
\item "perfekt" richtig $\implies$ gesucht
\end{enumerate}

\[\frac{1}{2}a t^2 + v_0 t = v_p (t - t_v)\]
\[\implies t_{1,2} = \frac{v_p - v_0 \pm \sqrt{(v_0 - v_p)^2 - 2 a v_p t_v}}{a}\]

\[(v_0 - v_p)^2 - 2 a v_p t_v = 0\]
$\rightarrow$ $v_p$

\[a t + v_0 = v_p \implies t = \frac{v_p - v_0}{a}\]
\[v_p = v_0 + at_v \pm \sqrt{(at_v + v_0)^2 - v_0^2} \approx \SI{11.9}{\meter\per\second}\]

\[x(t) = t v_{x0} = t v_0 \cos{\alpha}\]
\[y(t) = t v_0 \sin{\alpha} - \frac{1}{2}gt^2\]
\[x(T) = d\quad d = T v_0 \cos{\alpha} \implies t = \frac{d}{v_0 \cos{\alpha}}\]
\[y(T) = \frac{d \sin{\alpha}}{\cos{alpha}} - \frac{1}{2} g \frac{d^2}{v_0^2 \cos^2{\alpha}}\]
\[\implies v_0 = \sqrt{\frac{g d^2}{2\cos^2\alpha(d\tan\alpha - h)}}\]
\[\Delta h = \frac{D_L - D_B}{2}\]
\[v_0 = \sqrt{\frac{g d^2}{2\cos^2\alpha(a\tan \alpha - (h + \Delta h))}}\]
% Emacs 25.1.1 (Org mode 8.2.10)
\end{document}
